opentheory/haskell.ml
@@ -3,6 +3,313 @@
 (* Joe Hurd                                                                  *)
 (* ========================================================================= *)
 
+module String_map = Map.Make(String);;
+
+(***
+module Haskell =
+struct
+***)
+
+(* ------------------------------------------------------------------------- *)
+(* Haskell-in-HOL names.                                                     *)
+(* ------------------------------------------------------------------------- *)
+
+let mk_haskell_name s = s ^ "H";;
+
+let dest_haskell_name s =
+    let n = String.length s in
+    if n <= 1 then None else
+    if String.get s (n - 1) <> 'H' then None
+    else Some (String.sub s 0 (n - 1));;
+
+(* ------------------------------------------------------------------------- *)
+(* Haskell simplifications.                                                  *)
+(* ------------------------------------------------------------------------- *)
+
+type haskell_simp_thms =
+     Haskell_simp_thms of thm list;;
+
+let empty_haskell_simp_thms =
+    Haskell_simp_thms
+      [I_THM;
+       O_I;
+       I_O;
+       o_THM;
+       o_ASSOC'];;
+
+let add_haskell_simp_thm =
+    let o_thm = prove
+      (`!(f : B -> A) (g : C -> B) (h : C -> A).
+          f o g = h ==> !(j : Z -> C). f o (g o j) = h o j`,
+       REPEAT STRIP_TAC THEN
+       ASM_REWRITE_TAC [o_ASSOC]) in
+    let o_rule = GEN_ALL o MATCH_MP o_thm o SPEC_ALL in
+    fun st th ->
+      match st with
+        Haskell_simp_thms ths ->
+          let ths = th :: ths in
+          let ths =
+              try o_rule th :: ths
+              with Failure _ -> ths in
+          Haskell_simp_thms ths;;
+
+let add_haskell_simp_thms = List.fold_left add_haskell_simp_thm;;
+
+let haskell_simp_thms st =
+    match st with
+      Haskell_simp_thms ths -> ths;;
+
+let initial_haskell_simp_thms =
+    add_haskell_simp_thms empty_haskell_simp_thms
+    [MAP_I];;
+
+let the_haskell_thms = ref initial_haskell_simp_thms;;
+
+let add_haskell_thms ths =
+    let st = !the_haskell_thms in
+    let st = add_haskell_simp_thms st ths in
+    let () = the_haskell_thms := st in
+    ();;
+
+let add_haskell_thm th = add_haskell_thms [th];;
+
+let haskell_thms () =
+    let st = !the_haskell_thms in
+    haskell_simp_thms st;;
+
+let HASKELL_TAC ths goal = REWRITE_TAC (ths @ haskell_thms ()) goal;;
+
+(* ------------------------------------------------------------------------- *)
+(* Maintaining a mapping from HOL types to Haskell-in-HOL types.             *)
+(* ------------------------------------------------------------------------- *)
+
+type haskell_type_data =
+     {tyop : (string * string) option;
+      vars : (string * bool * bool) list};;
+
+type haskell_type_base =
+     Haskell_type_base of haskell_type_data String_map.t;;
+
+let empty_haskell_type_base =
+    Haskell_type_base String_map.empty;;
+
+let add_haskell_type_base tb (n,ld,vs) =
+    match tb with
+      Haskell_type_base m ->
+        let td = {tyop = ld; vars = vs} in
+        Haskell_type_base (String_map.add n td m);;
+
+let mem_haskell_type_base tb n =
+    match tb with
+      Haskell_type_base m ->
+        String_map.mem n m;;
+
+let find_haskell_type_base tb n =
+    match tb with
+      Haskell_type_base m ->
+        String_map.find n m;;
+
+let peek_haskell_type_base tb n =
+    if not (mem_haskell_type_base tb n) then None
+    else Some (find_haskell_type_base tb n);;
+
+let to_list_haskell_type_base tb =
+    match tb with
+      Haskell_type_base m ->
+        String_map.bindings m;;
+
+let lift_drop_haskell_type tb =
+    let mk_const_at_type (c,ty) =
+        let cty = get_const_type c in
+        let theta = type_match cty ty [] in
+        mk_const (c,theta) in
+    let mk_i ty =
+        let ity = mk_fun_ty ty ty in
+        mk_const_at_type ("I",ity) in
+    let mk_o (f,g) =
+        let fty = type_of f in
+        let (_,rng) = dest_fun_ty fty in
+        let gty = type_of g in
+        let (dom,_) = dest_fun_ty gty in
+        let oty = mk_fun_ty fty (mk_fun_ty gty (mk_fun_ty dom rng)) in
+        let otm = mk_const_at_type ("o",oty) in
+        mk_comb (mk_comb (otm,f), g) in
+    let list_mk_o fs =
+        match List.rev fs with
+          [] -> failwith "Haskell.lift_drop_haskell_type_base.list_mk_o: empty"
+        | f :: fs -> List.fold_left (fun t -> fun g -> mk_o (g,t)) f fs in
+    let rec lift ty =
+        if is_vartype ty then (ty,[]) else
+        let (ot,tys) = dest_type ty in
+        let () =
+            if mem_haskell_type_base tb ot then () else
+            failwith ("unknown type op: " ^ ot) in
+        let {tyop = ld; vars = vs} = find_haskell_type_base tb ot in
+        let (res,tysH) = lift_vars ty ot [] [] vs tys in
+        match ld with
+          None -> (mk_type (ot,tysH), res)
+        | Some (l,_) ->
+          let otH = mk_haskell_name ot in
+          let tyH = mk_type (otH,tysH) in
+          let lty = mk_fun_ty ty tyH in
+          let ltm = mk_const_at_type (l,lty) in
+          (tyH, ltm :: res)
+    and lift_vars pty ot res tysH vs tys =
+        match (vs,tys) with
+          ([],[]) -> (res, List.rev tysH)
+        | ([], _ :: _) -> failwith "Haskell.lift_drop_haskell_type.lift_vars"
+        | (_ :: _, []) -> failwith "Haskell.lift_drop_haskell_type.lift_vars"
+        | ((c,l,d) :: vs, ty :: tys) ->
+          let (tyH,lifts) = lift ty in
+          if List.length lifts = 0 then
+            lift_vars pty ot res (tyH :: tysH) vs tys
+          else
+            let pty' = mk_type (ot, List.rev tysH @ tyH :: tys) in
+            let cty =
+                let t = mk_fun_ty pty pty' in
+                let t = if d then mk_fun_ty (mk_fun_ty tyH ty) t else t in
+                let t = if l then mk_fun_ty (mk_fun_ty ty tyH) t else t in
+                t in
+            let ctm = mk_const_at_type (c,cty) in
+            let ctm =
+                if not l then ctm else
+                mk_comb (ctm, list_mk_o lifts) in
+            let ctm =
+                if not d then ctm else
+                let (_,drops) = drop tyH in
+                mk_comb (ctm, list_mk_o drops) in
+            lift_vars pty' ot (ctm :: res) (tyH :: tysH) vs tys
+    and drop tyH =
+        if is_vartype tyH then (tyH,[]) else
+        let (otH,tysH) = dest_type tyH in
+        let (ot,ld,vs) =
+            let (b,ot) =
+                match dest_haskell_name otH with
+                  Some ot -> (true,ot)
+                | None -> (false,otH) in
+            let () =
+                if mem_haskell_type_base tb ot then () else
+                failwith ("unknown type op: " ^ ot) in
+            let {tyop = ld; vars = vs} = find_haskell_type_base tb ot in
+            let () =
+                let b' =
+                    match ld with
+                      Some _ -> true
+                    | None -> false in
+                if b = b' then () else
+                failwith ("bad primitive type op: " ^ ot) in
+            (ot,ld,vs) in
+        let (pty,res) =
+            match ld with
+              None -> (tyH,[])
+            | Some (_,d) ->
+              let pty = mk_type (ot,tysH) in
+              let dty = mk_fun_ty tyH pty in
+              let dtm = mk_const_at_type (d,dty) in
+              (pty,[dtm]) in
+        let (res,tys) = drop_vars pty ot res [] (List.rev vs) (List.rev tysH) in
+        let ty = mk_type (ot,tys) in
+        (ty,res)
+    and drop_vars pty ot res tys vs tysH =
+        match (vs,tysH) with
+          ([],[]) -> (res,tys)
+        | ([], _ :: _) -> failwith "Haskell.lift_drop_haskell_type.drop_vars"
+        | (_ :: _, []) -> failwith "Haskell.lift_drop_haskell_type.drop_vars"
+        | ((c,l,d) :: vs, tyH :: tysH) ->
+          let (ty,drops) = drop tyH in
+          if List.length drops = 0 then
+            drop_vars pty ot res (ty :: tys) vs tysH
+          else
+            let pty' = mk_type (ot, List.rev tysH @ ty :: tys) in
+            let cty =
+                let t = mk_fun_ty pty pty' in
+                let t = if d then mk_fun_ty (mk_fun_ty ty tyH) t else t in
+                let t = if l then mk_fun_ty (mk_fun_ty tyH ty) t else t in
+                t in
+            let ctm = mk_const_at_type (c,cty) in
+            let ctm =
+                if not l then ctm else
+                mk_comb (ctm, list_mk_o drops) in
+            let ctm =
+                if not d then ctm else
+                let (_,lifts) = lift ty in
+                mk_comb (ctm, list_mk_o lifts) in
+            drop_vars pty' ot (ctm :: res) (ty :: tys) vs tysH in
+      let lift_ty ty =
+          let (tyH,lifts) = lift ty in
+          let tm =
+              if List.length lifts = 0 then mk_i ty else
+              list_mk_o lifts in
+          (tyH,tm) in
+      let drop_ty tyH =
+          let (ty,drops) = drop tyH in
+          let tm =
+              if List.length drops = 0 then mk_i tyH else
+              list_mk_o drops in
+          (ty,tm) in
+      (lift_ty,drop_ty);;
+
+let initial_haskell_type_base =
+    List.fold_left add_haskell_type_base empty_haskell_type_base
+    [("bool", None, []);
+     ("fun", None, [("map_domain", false, true); ("map_range", true, false)]);
+     ("list", None, [("MAP", true, false)]);
+     ("num", None, []);
+     ("option", None, [("map_option", true, false)]);
+     ("prod", None, [("map_fst", true, false); ("map_snd", true, false)]);
+     ("random", None, [])];;
+
+let the_haskell_type_base =
+    ref initial_haskell_type_base;;
+
+let haskell_types () =
+    to_list_haskell_type_base (!the_haskell_type_base);;
+
+let register_haskell_type (n,l,d,vs) =
+    let n =
+        match dest_haskell_name n with
+          None -> failwith ("not a haskell name: " ^ n)
+        | Some x -> x in
+    let tb = !the_haskell_type_base in
+    let tb = add_haskell_type_base tb (n, Some (l,d), vs) in
+    let () = the_haskell_type_base := tb in
+    ();;
+
+let define_haskell_type ty vs =
+    let (ot,tys) = dest_type ty in
+    let () =
+        if List.length tys = List.length vs then () else
+        failwith "define_haskell_type: bad variable list length" in
+    let otH = mk_haskell_name ot in
+    let mk n = "mkH_" ^ n in
+    let dest n = "destH_" ^ n in
+    let tybij = define_newtype' (mk,dest) ("h",otH) ("x",ty) in
+    let () = register_haskell_type (otH, mk otH, dest otH, vs) in
+    let () = add_haskell_thms (CONJUNCTS tybij) in
+    let () = add_haskell_thm (prove_newtype_inj tybij) in
+    tybij;;
+
+let lift_haskell_type ty =
+    let (lift,_) = lift_drop_haskell_type (!the_haskell_type_base) in
+    lift ty;;
+
+let drop_haskell_type tyH =
+    let (_,drop) = lift_drop_haskell_type (!the_haskell_type_base) in
+    drop tyH;;
+
+(* ------------------------------------------------------------------------- *)
+(* Maintaining a mapping from HOL constants to Haskell-in-HOL constants.     *)
+(* ------------------------------------------------------------------------- *)
+
+let define_haskell_const tm =
+    let (c,ty) = dest_const tm in
+    let cH = mk_haskell_name c in
+    let (tyH,ltm) = lift_haskell_type ty in
+    let def = mk_eq (mk_var (cH,tyH), mk_comb (ltm,tm)) in
+    let th = new_definition def in
+    let () = add_haskell_thm th in
+    th;;
+
 (* ------------------------------------------------------------------------- *)
 (* Haskellizing type variables in theorems.                                  *)
 (* ------------------------------------------------------------------------- *)
@@ -18,3 +325,13 @@ let haskellize_thm =
         INST_TYPE (List.fold_left mk_type_map [] vs) th;;
 
 let export_haskell_thm th = export_thm (haskellize_thm th);;
+
+(***
+end
+
+let define_haskell_type = Haskell.register_haskell_type
+and drop_haskell_type = Haskell.drop_haskell_type
+and export_haskell_thm = Haskell.export_haskell_thm
+and haskell_types = Haskell.haskell_types
+and lift_haskell_type = Haskell.lift_haskell_type;;
+***)
